1) removed 'ExitValue' from State, which was to denote the return value of 'main'. Actually this return result is already stored in the return insn on the top of the stack, because if a function stops, it must stop with the return insn as its last instruction (unless supporting 'invoke' to unwind stacks).
2) removed the cases that check if the recent stack is empty when return
is the current insn. These cases are too specific as inductive rules
(not strong enough for proofs). We can always check if there is only one
frame in the stack, and if the last insn on this frame is return to see
if we are reaching the final state.

3) Also commented out 'return void' to simply proofs, 'return typ value'
gives all interesting cases.

4) split transitivity-reflexivity closures into two cases: with 0, or
more steps -->*, and with at least one steps -->+. And generalized divergence
s -->* oo  as iff ex s', s.t. s -->+ s' /\ s -->* oo. (oo denotes
infinity, -->* oo is [dsop_diverges] in Coq), rather than ex s', s.t. s-->s' /\ s --->* oo. 

This change made coinductive proofs work at the following proof:
  if s ==> oo, then s -->* oo. where ==> is [dbopInf] in Coq.
s ==> oo gives s ==> s' and s' ==> oo.
By s ==> s' implies s -->+ s', we know s -->+ s'. With the new definion
of -->* oo, we conclude the proof by coinduction hypothesis, because
this CIH is used as one of arguments in this constructor, and satisfies
'Guarded' conditions. 

However, with the old definition, we have to complete the proof with
auxillary facts [trans]: s'' -->* s' /\ s' -->* oo -> s'' -->* oo, where
s --> s'' and s'' -->* s' by inversion on s -->+ s'. In this case,
by CIH, we have s' -->* oo. But s' -->* oo is first used in [trans], and
[trans] is used as one of the arguments of -->* oo. This fails 'Guarded'
checking in Coq, because it is hard to analyze the relations between CIH
results and constructors with [trans] in between.

5) Fixed the det-big-step cases "dbFdef" and "dbCallInsn", to match
small-steps, dbCallInsn calls dbFdef with the first insn in this
function on the top of the present stack ECs, as dbFdef' initial state,
and dbFdef stops when 'return' is the insn, and the returning stack is
ECs, finally the control returns back to dbCallInsn that gets the return
result, the new memory status by dbFdef, and then updates its memory
w.r.t the return result. This process exactly matches the sequence from
dsCallInsn to its matching dsReturn.

dbReturn was also removed, because we will never evalute 'return'
explicitly, that case is considered by 'dbCallInsn' when 'dbFdef' is
done.

also simplied rules.

7) the similar changes were done for non-deterministic rules, but with no
proofs and checkings.

8) Added tactics.v that defines cases notations for induction proofs

9) added opsem_conv.v that proved that bigsteps imply smallsteps when
convergence, going-wrong and divergence.




git-svn-id: https://webdav.seas.upenn.edu/svn/sol/vol@2473 eef5ea85-cc2e-0410-bd84-0fae1f012da8

src/ssa/ssa_dynamic.v
@@ -1,6 +1,9 @@
+Add LoadPath "./ott".
+Add LoadPath "./monads".
 Require Import ssa.
 Require Import List.
 Require Import Arith.
+Require Import tactics.
 
 Inductive GenericValue : Set := 
 | GV_int : forall (n:nat), GenericValue
@@ -20,7 +23,7 @@ fun i' =>
 Record ExecutionContext : Set := mkEC {
 CurFunction : fdef;
 CurBB       : block;
-CurInst     : insn;
+CurInsn     : insn;
 Locals      : GVMap;
 VarArgs     : list GenericValue
 }.
@@ -30,7 +33,6 @@ Definition ECStack := list ExecutionContext.
 Record State : Set := mkState {
 CurSystem   : system;
 CurModule   : module;
-ExistValue  : option GenericValue;
 ECS         : ECStack;
 Globals     : GVMap
 }.
@@ -61,7 +63,7 @@ Inductive wfExecutionContext : ExecutionContext -> Prop :=
   EC.(CurFunction) = fdef_intro fh lb ->
   In EC.(CurBB) lb ->
   EC.(CurBB) = block_intro l li ->
-  In EC.(CurInst) li ->
+  In EC.(CurInsn) li ->
   wfExecutionContext EC
 .
 
@@ -74,9 +76,9 @@ Inductive wfECStack : ECStack -> Prop :=
 .
 
 Inductive wfContexts : State -> Prop :=
-| wfContexts_intro : forall ECS ExistValue s m g,
+| wfContexts_intro : forall ECS s m g,
   wfECStack ECS ->
-  wfContexts (mkState s m ExistValue ECS g)
+  wfContexts (mkState s m ECS g)
 .
 
 Definition getCallerReturnID (Caller:insn) : option id :=
@@ -204,10 +206,10 @@ match v with
 | value_constant const_undef => Some GV_undef
 end.
 
-Fixpoint params2OpGenericValues (lp:list_param) (locals:GVMap) (globals:GVMap) : list (option GenericValue):=
+Fixpoint params2OpGVs (lp:list_param) (locals:GVMap) (globals:GVMap) : list (option GenericValue):=
 match lp with
 | nil => nil
-| (_, v)::lp' => getOperandValue v locals globals::params2OpGenericValues lp' locals globals
+| (_, v)::lp' => getOperandValue v locals globals::params2OpGVs lp' locals globals
 end.
 
 Fixpoint _initializeFrameValues (la:list_arg) (lg:list GenericValue) (locals:GVMap) : GVMap :=
@@ -216,17 +218,19 @@ match (la, lg) with
 | _ => locals
 end.
 
-Definition initializeFrameValues (la:list_arg) (lg:list GenericValue): GVMap := 
+Definition initLocals (la:list_arg) (lg:list GenericValue): GVMap := 
 _initializeFrameValues la lg (fun _ => None).
 
-Fixpoint opGenericValues2GenericValues (lg:list (option GenericValue)) : list GenericValue :=
+Fixpoint opGVs2GVs (lg:list (option GenericValue)) : list GenericValue :=
 match lg with
 | nil => nil
-| (Some g)::lg' => g::opGenericValues2GenericValues lg'
-| _::lg' => opGenericValues2GenericValues lg'
+| (Some g)::lg' => g::opGVs2GVs lg'
+| _::lg' => opGVs2GVs lg'
 end.
 
-Record Event : Set := mkEvent {}.
+Definition params2GVs (lp:list_param) (locals:GVMap) (globals:GVMap) := opGVs2GVs (params2OpGVs lp locals globals).
+
+Record Event : Set := mkEvent { }.
 
 Inductive trace : Set :=
 | trace_nil : trace
@@ -237,67 +241,50 @@ CoInductive Trace : Set :=
 | Trace_cons : Event -> Trace -> Trace
 .
 
-Fixpoint trace_app (t1 t2:trace) : trace :=
-match t1 with
-| trace_nil => t2
-| trace_cons t t1' => trace_cons t (trace_app t1' t2)
+Fixpoint trace_app (tr1 tr2:trace) : trace :=
+match tr1 with
+| trace_nil => tr2
+| trace_cons e tr1' => trace_cons e (trace_app tr1' tr2)
 end.
 
-Fixpoint Trace_app (t1:trace) (t2:Trace) : Trace :=
-match t1 with
-| trace_nil => t2
-| trace_cons t t1' => Trace_cons t (Trace_app t1' t2)
+Fixpoint Trace_app (tr1:trace) (tr2:Trace) : Trace :=
+match tr1 with
+| trace_nil => tr2
+| trace_cons e tr1' => Trace_cons e (Trace_app tr1' tr2)
 end.
 
 (***************************************************************)
 (* deterministic small-step *)
 
-Inductive dsInst : State -> State -> trace -> Prop :=
-| dsReturn_finished : forall S M F B RetTy Result lc gl arg ExitValue,
-  (* Finished main.  Put result into exit code... *)
-  ExitValue =  (if (Typ.isInteger RetTy)  (* Nonvoid return type? *)
-               then getOperandValue Result lc gl (* Capture the exit value of the program *)
-               else Some GV_undef) ->
-  dsInst 
-    (mkState S M None ((mkEC F B (insn_return RetTy Result) lc arg)::nil) gl)
-    (mkState S M ExitValue nil gl)
-    trace_nil 
-| dsReturn_call : forall S M F B RetTy Result lc gl arg id
-                            F' B' I' lc' arg' EC gv
+Inductive dsInsn : State -> State -> trace -> Prop :=
+| dsReturn : forall S M F B RetTy Result lc gl arg id
+                            F' B' I' lc' arg' EC
                             I'' lc'' gl'',   
   (* If we have a previous stack frame, and we have a previous call,
           fill in the return value... *)
-  Instruction.isCallInst I' ->
+  Instruction.isCallInst I' = true ->
   getCallerReturnID I' = Some id ->
-  getOperandValue Result lc gl = Some gv -> 
   (lc'', gl'') = (if (RetTy =t= typ_void) 
                   then (lc', gl) 
-                  else (updateMem lc' gl id (Some gv))) ->
+                  else (updateMem lc' gl id (getOperandValue Result lc gl))) ->
   getNextInsnFrom I' B' = Some I'' ->
-  dsInst 
-    (mkState S M None ((mkEC F B (insn_return RetTy Result) lc arg)::(mkEC F' B' I' lc' arg')::EC) gl)
-    (mkState S M None ((mkEC F' B' I'' lc'' arg')::EC) gl'')
+  dsInsn 
+    (mkState S M ((mkEC F B (insn_return RetTy Result) lc arg)::(mkEC F' B' I' lc' arg')::EC) gl)
+    (mkState S M ((mkEC F' B' I'' lc'' arg')::EC) gl'')
     trace_nil 
-| dsReturnVoid_finished : forall S M F B lc gl arg ExitValue,
-  (* Finished main.  Put result into exit code... *)
-  ExitValue = Some GV_undef ->
-  dsInst 
-    (mkState S M None ((mkEC F B (insn_return_void) lc arg)::nil) gl)
-    (mkState S M ExitValue nil gl)
-    trace_nil
-| dsReturnVoid_call : forall S M F B lc gl arg ExitValue id
+(*
+| dsReturnVoid : forall S M F B lc gl arg id
                             F' B' I' lc' arg' EC
                             I'',   
-  (* If we have a previous stack frame, and we have a previous call,
-          fill in the return value... *)
-  Instruction.isCallInst I' ->
+  Instruction.isCallInst I' = true ->
   getCallerReturnID I' = Some id ->
   getNextInsnFrom I' B' = Some I'' ->
-  dsInst 
-    (mkState S M ExitValue ((mkEC F B insn_return_void lc arg)::(mkEC F' B' I' lc' arg')::EC) gl)
-    (mkState S M ExitValue ((mkEC F' B' I'' lc' arg')::EC) gl)
+  dsInsn 
+    (mkState S M ((mkEC F B insn_return_void lc arg)::(mkEC F' B' I' lc' arg')::EC) gl)
+    (mkState S M ((mkEC F' B' I'' lc' arg')::EC) gl)
     trace_nil 
-| dsBranch : forall S M F B lc gl arg ExitValue t Cond l1 l2 c
+*)
+| dsBranch : forall S M F B lc gl arg t Cond l1 l2 c
                               B' I' lc' Dest EC,   
   getOperandValue Cond lc gl = Some (GV_int c) ->
   Some Dest = (if c 
@@ -305,40 +292,39 @@ Inductive dsInst : State -> State -> trace -> Prop :=
                else lookupBlockViaLabelFromSystem S l2) ->
   (B', lc') = (switchToNewBasicBlock Dest B lc) ->
   getEntryInsn B' = Some I' ->
-  dsInst 
-    (mkState S M ExitValue ((mkEC F B (insn_br t Cond l1 l2) lc arg)::EC) gl)
-    (mkState S M ExitValue ((mkEC F B' I' lc' arg)::EC) gl)
+  dsInsn 
+    (mkState S M ((mkEC F B (insn_br t Cond l1 l2) lc arg)::EC) gl)
+    (mkState S M ((mkEC F B' I' lc' arg)::EC) gl)
     trace_nil 
-| dsBranch_uncond : forall S M F B lc gl arg ExitValue l
+| dsBranch_uncond : forall S M F B lc gl arg l
                               B' I' lc' Dest EC,   
   Some Dest = (lookupBlockViaLabelFromSystem S l) ->
   (B', lc') = (switchToNewBasicBlock Dest B lc) ->
   getEntryInsn B = Some I' ->
-  dsInst 
-    (mkState S M ExitValue ((mkEC F B (insn_br_uncond l) lc arg)::EC) gl)
-    (mkState S M ExitValue ((mkEC F B' I' lc' arg)::EC) gl)
+  dsInsn 
+    (mkState S M ((mkEC F B (insn_br_uncond l) lc arg)::EC) gl)
+    (mkState S M ((mkEC F B' I' lc' arg)::EC) gl)
     trace_nil 
-| dsCallInsnt : forall S M F B lc gl arg ExitValue rid t fid lp
-                            Oparg' arg' F' B' I' EC rt id la lb lc',
-  params2OpGenericValues lp lc gl = Oparg' ->   
-  opGenericValues2GenericValues Oparg' = arg' ->   
-  lookupFdefViaIDFromSystemC S fid = Some F' ->
-  getEntryBlock F' = Some B' ->
+| dsCallInsn : forall S M F B lc gl arg rid fid lp
+                            B' I' EC rt la lb,
+  lookupFdefViaIDFromSystemC S fid = Some (fdef_intro (fheader_intro rt fid la) lb) ->
+  getEntryBlock (fdef_intro (fheader_intro rt fid la) lb) = Some B' ->
   getEntryInsn B' = Some I' ->
-  F' = fdef_intro (fheader_intro rt id la) lb ->
-  initializeFrameValues la arg' = lc' ->
-  dsInst 
-    (mkState S M ExitValue ((mkEC F B (insn_call rid t fid lp) lc arg)::EC) gl)
-    (mkState S M ExitValue ((mkEC F' B' I' lc' arg')::(mkEC F B (insn_call rid t fid lp) lc arg)::EC) gl)
+  dsInsn 
+    (mkState S M ((mkEC F B (insn_call rid rt fid lp) lc arg)::EC) gl)
+    (mkState S M ((mkEC (fdef_intro (fheader_intro rt fid la) lb) 
+                             B' I' (initLocals la (params2GVs lp lc gl)) 
+                             (params2GVs lp lc gl))::
+                       (mkEC F B (insn_call rid rt fid lp) lc arg)::EC) gl)
     trace_nil 
-| dsAddInsnt : forall S M F B lc gl lc' gl' arg ExitValue id t v1 v2 EC i1 i2 I',
+| dsAddInsn : forall S M F B lc gl lc' gl' arg id t v1 v2 EC i1 i2 I',
   getOperandValue v1 lc gl = Some (GV_int i1) ->
   getOperandValue v2 lc gl = Some (GV_int i2) ->
   getNextInsnFrom (insn_add id t v1 v2) B = Some I' ->
   updateMem lc gl id (Some (GV_int (i1+i2))) = (lc', gl') -> 
-  dsInst 
-    (mkState S M ExitValue ((mkEC F B (insn_add id t v1 v2) lc arg)::EC) gl) 
-    (mkState S M ExitValue ((mkEC F B I' lc' arg)::EC) gl')
+  dsInsn 
+    (mkState S M ((mkEC F B (insn_add id t v1 v2) lc arg)::EC) gl) 
+    (mkState S M ((mkEC F B I' lc' arg)::EC) gl')
     trace_nil 
 .
 
@@ -360,12 +346,11 @@ match (lookupFdefViaIDFromSystemC S main) with
       | Some CurInst =>
         match CurFunction with 
         | fdef_intro (fheader_intro rt _ la) _ =>
-          let Values := initializeFrameValues la VarArgs in
+          let Values := initLocals la VarArgs in
           Some
             (mkState
               S
               CurModule
-              None
               ((mkEC
                 CurFunction 
                 CurBB 
@@ -381,47 +366,54 @@ match (lookupFdefViaIDFromSystemC S main) with
   end
 end.
 
-Definition ds_isFinialState (S:State) : bool :=
-match S with
-| (mkState _ _ _ nil _) => true
+Definition ds_isFinialState (state:State) : bool :=
+match state with
+| (mkState _ _ ((mkEC _ _ insn_return_void _ _ )::nil) _) => true
+(* | (mkState _ _ ((mkEC _ _ (insn_return _ _) _ _)::nil) _) => true *)
 | _ => false
 end.
 
-Inductive dsop : State -> State -> trace -> Prop :=
-| dsop_nil : forall S, dsop S S trace_nil
-| dsop_cons : forall S1 S2 S3 t1 t2,
-    dsInst S1 S2 t1 ->
-    dsop S2 S3 t2 ->
-    dsop S1 S3 (trace_app t1 t2)
+Inductive dsop_star : State -> State -> trace -> Prop :=
+| dsop_star_nil : forall state, dsop_star state state trace_nil
+| dsop_star_cons : forall state1 state2 state3 tr1 tr2,
+    dsInsn state1 state2 tr1 ->
+    dsop_star state2 state3 tr2 ->
+    dsop_star state1 state3 (trace_app tr1 tr2)
 .
 
-CoInductive dsop_diverges : State -> State -> Trace -> Prop :=
-| dsop_diverges_intro : forall S1 S2 S3 t1 t2,
-    dsInst S1 S2 t1 ->
-    dsop_diverges S2 S3 t2 ->
-    dsop_diverges S1 S3 (Trace_app t1 t2)
+Inductive dsop_plus : State -> State -> trace -> Prop :=
+| dsop_plus_cons : forall state1 state2 state3 tr1 tr2,
+    dsInsn state1 state2 tr1 ->
+    dsop_star state2 state3 tr2 ->
+    dsop_plus state1 state3 (trace_app tr1 tr2)
+.
+
+CoInductive dsop_diverges : State -> Trace -> Prop :=
+| dsop_diverges_intro : forall state1 state2 tr1 tr2,
+    dsop_plus state1 state2 tr1 ->
+    dsop_diverges state2 tr2 ->
+    dsop_diverges state1 (Trace_app tr1 tr2)
 .
 
 Inductive ds_converges : system -> id -> list GenericValue -> State -> Prop :=
 | ds_converges_intro : forall (s:system) (main:id) (VarArgs:list GenericValue) (IS FS:State) tr,
   ds_genInitState s main VarArgs = Some IS ->
-  dsop IS FS tr ->
+  dsop_star IS FS tr ->
   ds_isFinialState FS ->
   ds_converges s main VarArgs FS
 .
 
 Inductive ds_diverges : system -> id -> list GenericValue -> Prop :=
-| ds_diverges_intro : forall (s:system) (main:id) (VarArgs:list GenericValue) (IS S:State) tr,
+| ds_diverges_intro : forall (s:system) (main:id) (VarArgs:list GenericValue) (IS:State) tr,
   ds_genInitState s main VarArgs = Some IS ->
-  dsop_diverges IS S tr ->
+  dsop_diverges IS tr ->
   ds_diverges s main VarArgs
 .
-
 
 Inductive ds_goeswrong : system -> id -> list GenericValue -> State -> Prop :=
 | ds_goeswrong_intro : forall (s:system) (main:id) (VarArgs:list GenericValue) (IS FS:State) tr,
   ds_genInitState s main VarArgs = Some IS ->
-  dsop IS FS tr ->
+  dsop_star IS FS tr ->
   ~ ds_isFinialState FS ->
   ds_goeswrong s main VarArgs FS
 .
@@ -436,54 +428,39 @@ Definition States := list (State*trace).
 
 Inductive wfStates : States -> Prop :=
 | wfStates_nil : wfStates nil
-| wfStates_cons : forall state t states,
+| wfStates_cons : forall state te states,
   wfState state ->
   wfStates states ->
-  wfStates ((state, t)::states)
+  wfStates ((state, te)::states)
 .
 
-Inductive nsInst : State*trace -> States -> Prop :=
-| nsReturn_finished : forall S M F B RetTy Result lc gl arg ExitValue tr,
-  (* Finished main.  Put result into exit code... *)
-  ExitValue =  (if (Typ.isInteger RetTy)  (* Nonvoid return type? *)
-               then getOperandValue Result lc gl (* Capture the exit value of the program *)
-               else Some GV_undef) ->
-  nsInst 
-    (mkState S M None ((mkEC F B (insn_return RetTy Result) lc arg)::nil) gl, tr)
-    ((mkState S M ExitValue nil gl, tr)::nil)
-| nsReturn_call : forall S M F B RetTy Result lc gl arg id
-                            F' B' I' lc' arg' EC gv
+Inductive nsInsn : State*trace -> States -> Prop :=
+| nsReturn : forall S M F B RetTy Result lc gl arg id
+                            F' B' I' lc' arg' EC
                             I'' lc'' gl'' tr,   
   (* If we have a previous stack frame, and we have a previous call,
           fill in the return value... *)
-  Instruction.isCallInst I' ->
+  Instruction.isCallInst I' = true ->
   getCallerReturnID I' = Some id ->
-  getOperandValue Result lc gl = Some gv -> 
   (lc'', gl'') = (if (RetTy =t= typ_void) 
                   then (lc', gl) 
-                  else (updateMem lc' gl id (Some gv))) ->
+                  else (updateMem lc' gl id (getOperandValue Result lc gl))) ->
   getNextInsnFrom I' B' = Some I'' ->
-  nsInst 
-    (mkState S M None ((mkEC F B (insn_return RetTy Result) lc arg)::(mkEC F' B' I' lc' arg')::EC) gl, tr)
-    ((mkState S M None ((mkEC F' B' I'' lc'' arg')::EC) gl'', tr)::nil)
-| nsReturnVoid_finished : forall S M F B lc gl arg ExitValue tr,
-  (* Finished main.  Put result into exit code... *)
-  ExitValue = Some GV_undef ->
-  nsInst 
-    (mkState S M None ((mkEC F B (insn_return_void) lc arg)::nil) gl, tr)
-    ((mkState S M ExitValue nil gl, tr)::nil)
-| nsReturnVoid_call : forall S M F B lc gl arg ExitValue id
+  nsInsn 
+    (mkState S M ((mkEC F B (insn_return RetTy Result) lc arg)::(mkEC F' B' I' lc' arg')::EC) gl, tr)
+    ((mkState S M ((mkEC F' B' I'' lc'' arg')::EC) gl'', tr)::nil)
+(* 
+| nsReturnVoid : forall S M F B lc gl arg id
                             F' B' I' lc' arg' EC
                             I'' tr,   
-  (* If we have a previous stack frame, and we have a previous call,
-          fill in the return value... *)
-  Instruction.isCallInst I' ->
+  Instruction.isCallInst I' = true ->
   getCallerReturnID I' = Some id ->
   getNextInsnFrom I' B' = Some I'' ->
-  nsInst 
-    (mkState S M ExitValue ((mkEC F B insn_return_void lc arg)::(mkEC F' B' I' lc' arg')::EC) gl, tr)
-    ((mkState S M ExitValue ((mkEC F' B' I'' lc' arg')::EC) gl, tr)::nil)
-| nsBranch_def : forall S M F B lc gl arg ExitValue t Cond l1 l2 c
+  nsInsn 
+    (mkState S M ((mkEC F B insn_return_void lc arg)::(mkEC F' B' I' lc' arg')::EC) gl, tr)
+    ((mkState S M ((mkEC F' B' I'' lc' arg')::EC) gl, tr)::nil)
+*)
+| nsBranch_def : forall S M F B lc gl arg t Cond l1 l2 c
                               B' I' lc' Dest EC tr,   
   getOperandValue Cond lc gl = Some (GV_int c) ->
   Some Dest = (if c 
@@ -491,10 +468,10 @@ Inductive nsInst : State*trace -> States -> Prop :=
                else lookupBlockViaLabelFromSystem S l2) ->
   (B', lc') = (switchToNewBasicBlock Dest B lc) ->
   getEntryInsn B' = Some I' ->
-  nsInst 
-    (mkState S M ExitValue ((mkEC F B (insn_br t Cond l1 l2) lc arg)::EC) gl, tr)
-    ((mkState S M ExitValue ((mkEC F B' I' lc' arg)::EC) gl, tr)::nil)
-| nsBranch_undef : forall S M F B lc arg ExitValue t Cond l1 l2
+  nsInsn 
+    (mkState S M ((mkEC F B (insn_br t Cond l1 l2) lc arg)::EC) gl, tr)
+    ((mkState S M ((mkEC F B' I' lc' arg)::EC) gl, tr)::nil)
+| nsBranch_undef : forall S M F B lc arg t Cond l1 l2
                               B1' I1' lc1' B2' I2' lc2' Dest1 Dest2 EC gl tr,   
   getOperandValue Cond lc gl = Some GV_undef ->
   Some Dest1 = lookupBlockViaLabelFromSystem S l1 ->
@@ -503,38 +480,38 @@ Inductive nsInst : State*trace -> States -> Prop :=
   (B2', lc2') = (switchToNewBasicBlock Dest2 B lc) ->
   getEntryInsn B1' = Some I1' ->
   getEntryInsn B2' = Some I2' ->
-  nsInst 
-    (mkState S M ExitValue ((mkEC F B (insn_br t Cond l1 l2) lc arg)::EC) gl, tr)
-    ((mkState S M ExitValue ((mkEC F B1' I1' lc1' arg)::EC) gl, tr)::
-     (mkState S M ExitValue ((mkEC F B2' I2' lc2' arg)::EC) gl, tr)::nil)
-| nsBranch_uncond : forall S M F B lc gl arg ExitValue l
+  nsInsn 
+    (mkState S M ((mkEC F B (insn_br t Cond l1 l2) lc arg)::EC) gl, tr)
+    ((mkState S M ((mkEC F B1' I1' lc1' arg)::EC) gl, tr)::
+     (mkState S M ((mkEC F B2' I2' lc2' arg)::EC) gl, tr)::nil)
+| nsBranch_uncond : forall S M F B lc gl arg l
                               B' I' lc' Dest EC tr,   
   Some Dest = (lookupBlockViaLabelFromSystem S l) ->
   (B', lc') = (switchToNewBasicBlock Dest B lc) ->
   getEntryInsn B = Some I' ->
-  nsInst 
-    (mkState S M ExitValue ((mkEC F B (insn_br_uncond l) lc arg)::EC) gl, tr)
-    ((mkState S M ExitValue ((mkEC F B' I' lc' arg)::EC) gl, tr)::nil)
-| nsCallInsnt : forall S M F B lc gl arg ExitValue rid t fid lp
+  nsInsn 
+    (mkState S M ((mkEC F B (insn_br_uncond l) lc arg)::EC) gl, tr)
+    ((mkState S M ((mkEC F B' I' lc' arg)::EC) gl, tr)::nil)
+| nsCallInsn : forall S M F B lc gl arg rid fid lp
                             Oparg' arg' F' B' I' EC rt id la lb lc' tr,
-  params2OpGenericValues lp lc gl = Oparg' ->   
-  opGenericValues2GenericValues Oparg' = arg' ->   
+  params2OpGVs lp lc gl = Oparg' ->   
+  opGVs2GVs Oparg' = arg' ->   
   lookupFdefViaIDFromSystemC S fid = Some F' ->
   getEntryBlock F' = Some B' ->
   getEntryInsn B' = Some I' ->
   F' = fdef_intro (fheader_intro rt id la) lb ->
-  initializeFrameValues la arg' = lc' ->
-  nsInst 
-    (mkState S M ExitValue ((mkEC F B (insn_call rid t fid lp) lc arg)::EC) gl, tr)
-    ((mkState S M ExitValue ((mkEC F' B' I' lc' arg')::(mkEC F B (insn_call rid t fid lp) lc arg)::EC) gl, tr)::nil)
-| nsAddInsnt : forall S M F B lc gl lc' gl' arg ExitValue id t v1 v2 EC i1 i2 I' tr,
+  initLocals la arg' = lc' ->
+  nsInsn 
+    (mkState S M ((mkEC F B (insn_call rid rt fid lp) lc arg)::EC) gl, tr)
+    ((mkState S M ((mkEC F' B' I' lc' arg')::(mkEC F B (insn_call rid rt fid lp) lc arg)::EC) gl, tr)::nil)
+| nsAddInsn : forall S M F B lc gl lc' gl' arg id t v1 v2 EC i1 i2 I' tr,
   getOperandValue v1 lc gl = Some (GV_int i1) ->
   getOperandValue v2 lc gl = Some (GV_int i2) ->
   getNextInsnFrom (insn_add id t v1 v2) B = Some I' ->
   updateMem lc gl id (Some (GV_int (i1+i2))) = (lc', gl') -> 
-  nsInst 
-    (mkState S M ExitValue ((mkEC F B (insn_add id t v1 v2) lc arg)::EC) gl, tr) 
-    ((mkState S M ExitValue ((mkEC F B I' lc' arg)::EC) gl', tr)::nil)
+  nsInsn 
+    (mkState S M ((mkEC F B (insn_add id t v1 v2) lc arg)::EC) gl, tr) 
+    ((mkState S M ((mkEC F B I' lc' arg)::EC) gl', tr)::nil)
 .
 
 Definition ns_genInitState (S:system) (main:id) (VarArgs:list GenericValue) : option States :=
@@ -552,12 +529,11 @@ match (lookupFdefViaIDFromSystemC S main) with
       | Some CurInst =>
         match CurFunction with 
         | fdef_intro (fheader_intro rt _ la) _ =>
-          let Values := initializeFrameValues la VarArgs in
+          let Values := initLocals la VarArgs in
           Some
             ((mkState
               S
               CurModule
-              None
               ((mkEC
                 CurFunction 
                 CurBB 
@@ -576,53 +552,65 @@ end.
 
 Fixpoint ns_isFinialState (states:States) : bool :=
 match states with
-| (mkState _ _ _ nil _, _)::states' => true
-| (mkState _ _ _ _ _, _)::states' => ns_isFinialState states'
+| (mkState _ _ ((mkEC _ _ insn_return_void _ _ )::nil) _, _)::states' => true
+(* | (mkState _ _ ((mkEC _ _ (insn_return _ _) _ _)::nil) _, _)::states' => true *)
+| (mkState _ _ _ _, _)::states' => ns_isFinialState states'
 | _ => false
 end.
 
-Inductive nsInstMerge : States -> States -> Prop :=
-| nsInstMerge_nil : nsInstMerge nil nil
-| nsInstMerge_cons : forall state tr states states1 states2,
-  nsInst (state, tr) states1 ->
-  nsInstMerge states states2 ->
-  nsInstMerge ((state, tr)::states) (states1++states2)
+Inductive nsInsnMerge : States -> States -> Prop :=
+| nsInsnMerge_nil : nsInsnMerge nil nil
+| nsInsnMerge_cons : forall state tr states states1 states2,
+  nsInsn (state, tr) states1 ->
+  nsInsnMerge states states2 ->
+  nsInsnMerge ((state, tr)::states) (states1++states2)
+| nssnsnMerge_final : forall state tr states states',
+  ds_isFinialState state ->
+  nsInsnMerge states states' ->
+  nsInsnMerge ((state, tr)::states) ((state, tr)::states')
 .
 
-Inductive nsop : States -> States -> Prop :=
-| nsop_nil : nsop nil nil
-| nsop_cons : forall states1 states2 states3,
-  nsInstMerge states1 states2 ->
-  nsop states2 states3 ->
-  nsop states1 states3
+Inductive nsop_star : States -> States -> Prop :=
+| nsop_star_nil : nsop_star nil nil
+| nsop_star_cons : forall states1 states2 states3,
+  nsInsnMerge states1 states2 ->
+  nsop_star states2 states3 ->
+  nsop_star states1 states3
 .
 
-CoInductive nsop_diverges : States -> States -> Prop :=
-| nsop_diverges_intro : forall state tr states states1 states2,
-    nsInst (state,tr) states1 ->
-    nsop_diverges states states2 ->
-    nsop_diverges ((state, tr)::states) (states1++states2)
+Inductive nsop_plus : States -> States -> Prop :=
+| nsop_plus_cons : forall states1 states2 states3,
+  nsInsnMerge states1 states2 ->
+  nsop_plus states2 states3 ->
+  nsop_plus states1 states3
+.
+
+CoInductive nsop_diverges : States -> Prop :=
+| nsop_diverges_intro : forall states states',
+    nsop_plus states states' ->
+    nsop_diverges states' ->
+    nsop_diverges states
 .
 
 Inductive ns_converges : system -> id -> list GenericValue -> States -> Prop :=
 | ns_converges_intro : forall (s:system) (main:id) (VarArgs:list GenericValue) (IS FS:States),
   ns_genInitState s main VarArgs = Some IS ->
-  nsop IS FS ->
+  nsop_star IS FS ->
   ns_isFinialState FS ->
   ns_converges s main VarArgs FS
 .
 
 Inductive ns_diverges : system -> id -> list GenericValue -> Prop :=
-| ns_diverges_intro : forall (s:system) (main:id) (VarArgs:list GenericValue) (IS S:States),
+| ns_diverges_intro : forall (s:system) (main:id) (VarArgs:list GenericValue) (IS:States),
   ns_genInitState s main VarArgs = Some IS ->
-  nsop_diverges IS S ->
+  nsop_diverges IS ->
   ns_diverges s main VarArgs
 .
 
 Inductive ns_goeswrong : system -> id -> list GenericValue -> States -> Prop :=
 | ns_goeswrong_intro : forall (s:system) (main:id) (VarArgs:list GenericValue) (IS FS:States),
   ns_genInitState s main VarArgs = Some IS ->
-  nsop IS FS ->
+  nsop_star IS FS ->
   ~ ns_isFinialState FS ->
   ns_goeswrong s main VarArgs FS
 .
@@ -630,52 +618,8 @@ Inductive ns_goeswrong : system -> id -> list GenericValue -> States -> Prop :=
 (***************************************************************)
 (* deterministic big-step *)
 
-Inductive dbInst : State -> State -> trace -> Prop :=
-| dbReturn_finished : forall S M F B RetTy Result lc gl arg ExitValue,
-  (* Finished main.  Put result into exit code... *)
-  ExitValue =  (if (Typ.isInteger RetTy)  (* Nonvoid return type? *)
-               then getOperandValue Result lc gl (* Capture the exit value of the program *)
-               else Some GV_undef) ->
-  dbInst 
-    (mkState S M None ((mkEC F B (insn_return RetTy Result) lc arg)::nil) gl)
-    (mkState S M ExitValue nil gl)
-    trace_nil 
-| dbReturn_call : forall S M F B RetTy Result lc gl arg id
-                            F' B' I' lc' arg' EC gv
-                            I'' lc'' gl'',   
-  (* If we have a previous stack frame, and we have a previous call,
-          fill in the return value... *)
-  Instruction.isCallInst I' ->
-  getCallerReturnID I' = Some id ->
-  getOperandValue Result lc gl = Some gv -> 
-  (lc'', gl'') = (if (RetTy =t= typ_void) 
-                  then (lc', gl) 
-                  else (updateMem lc' gl id (Some gv))) ->
-  getNextInsnFrom I' B' = Some I'' ->
-  dbInst 
-    (mkState S M None ((mkEC F B (insn_return RetTy Result) lc arg)::(mkEC F' B' I' lc' arg')::EC) gl)
-    (mkState S M None ((mkEC F' B' I'' lc'' arg')::EC) gl'')
-    trace_nil 
-| dbReturnVoid_finished : forall S M F B lc gl arg ExitValue,
-  (* Finished main.  Put result into exit code... *)
-  ExitValue = Some GV_undef ->
-  dbInst 
-    (mkState S M None ((mkEC F B (insn_return_void) lc arg)::nil) gl)
-    (mkState S M ExitValue nil gl)
-    trace_nil
-| dbReturnVoid_call : forall S M F B lc gl arg ExitValue id
-                            F' B' I' lc' arg' EC
-                            I'',   
-  (* If we have a previous stack frame, and we have a previous call,
-          fill in the return value... *)
-  Instruction.isCallInst I' ->
-  getCallerReturnID I' = Some id ->
-  getNextInsnFrom I' B' = Some I'' ->
-  dbInst 
-    (mkState S M ExitValue ((mkEC F B insn_return_void lc arg)::(mkEC F' B' I' lc' arg')::EC) gl)
-    (mkState S M ExitValue ((mkEC F' B' I'' lc' arg')::EC) gl)
-    trace_nil 
-| dbBranch : forall S M F B lc gl arg ExitValue t Cond l1 l2 c
+Inductive dbInsn : State -> State -> trace -> Prop :=
+| dbBranch : forall S M F B lc gl arg t Cond l1 l2 c
                               B' I' lc' Dest EC,   
   getOperandValue Cond lc gl = Some (GV_int c) ->
   Some Dest = (if c 
@@ -683,99 +627,90 @@ Inductive dbInst : State -> State -> trace -> Prop :=
                else lookupBlockViaLabelFromSystem S l2) ->
   (B', lc') = (switchToNewBasicBlock Dest B lc) ->
   getEntryInsn B' = Some I' ->
-  dbInst 
-    (mkState S M ExitValue ((mkEC F B (insn_br t Cond l1 l2) lc arg)::EC) gl)
-    (mkState S M ExitValue ((mkEC F B' I' lc' arg)::EC) gl)
+  dbInsn 
+    (mkState S M ((mkEC F B (insn_br t Cond l1 l2) lc arg)::EC) gl)
+    (mkState S M ((mkEC F B' I' lc' arg)::EC) gl)
     trace_nil 
-| dbBranch_uncond : forall S M F B lc gl arg ExitValue l
+| dbBranch_uncond : forall S M F B lc gl arg l
                               B' I' lc' Dest EC,   
   Some Dest = (lookupBlockViaLabelFromSystem S l) ->
   (B', lc') = (switchToNewBasicBlock Dest B lc) ->
   getEntryInsn B = Some I' ->
-  dbInst 
-    (mkState S M ExitValue ((mkEC F B (insn_br_uncond l) lc arg)::EC) gl)
-    (mkState S M ExitValue ((mkEC F B' I' lc' arg)::EC) gl)
+  dbInsn 
+    (mkState S M ((mkEC F B (insn_br_uncond l) lc arg)::EC) gl)
+    (mkState S M ((mkEC F B' I' lc' arg)::EC) gl)
     trace_nil 
-| dbCallInsnt : forall S M F B lc gl arg rid t fid lp gl' gl''
-                       EC ExitValue ReturnValue tr I',
-  dbFdef fid lp
-    (mkState S M None ((mkEC F B (insn_call rid t fid lp) lc arg)::nil) gl) 
-    (mkState S M ReturnValue nil gl') 
-    tr ->
-  updateGlobals gl' rid ReturnValue = gl'' -> 
-  getNextInsnFrom (insn_call rid t fid lp) B = Some I' ->
-  dbInst 
-    (mkState S M ExitValue ((mkEC F B (insn_call rid t fid lp) lc arg)::EC) gl) 
-    (mkState S M ExitValue ((mkEC F B I' lc arg)::EC) gl'') 
+| dbCallInsn : forall S M F B lc gl arg rid rt fid lp gl' gl''
+                       EC Result tr I' lc'' B' lc' oGV,
+  dbFdef fid rt lp S M ((mkEC F B (insn_call rid rt fid lp) lc arg)::EC) lc gl lc' gl' B' Result tr ->
+  getOperandValue Result lc' gl' = oGV -> 
+  (lc'', gl'') = (if (rt =t= typ_void) 
+                  then (lc, gl') 
+                  else (updateMem lc gl' rid oGV)) ->
+  getNextInsnFrom (insn_call rid rt fid lp) B = Some I' ->
+  dbInsn 
+    (mkState S M ((mkEC F B (insn_call rid rt fid lp) lc arg)::EC) gl) 
+    (mkState S M ((mkEC F B I' lc'' arg)::EC) gl'') 
     tr
-| dbAddInsnt : forall S M F B lc gl lc' gl' arg ExitValue id t v1 v2 EC i1 i2 I',
+| dbAddInsn : forall S M F B lc gl lc' gl' arg id t v1 v2 EC i1 i2 I',
   getOperandValue v1 lc gl = Some (GV_int i1) ->
   getOperandValue v2 lc gl = Some (GV_int i2) ->
   getNextInsnFrom (insn_add id t v1 v2) B = Some I' ->
   updateMem lc gl id (Some (GV_int (i1+i2))) = (lc', gl') -> 
-  dbInst 
-    (mkState S M ExitValue ((mkEC F B (insn_add id t v1 v2) lc arg)::EC) gl) 
-    (mkState S M ExitValue ((mkEC F B I' lc' arg)::EC) gl')
+  dbInsn 
+    (mkState S M ((mkEC F B (insn_add id t v1 v2) lc arg)::EC) gl) 
+    (mkState S M ((mkEC F B I' lc' arg)::EC) gl')
     trace_nil 
 with dbop : State -> State -> trace -> Prop :=
 | dbop_nil : forall S, dbop S S trace_nil
 | dbop_cons : forall S1 S2 S3 t1 t2,
-    dbInst S1 S2 t1 ->
+    dbInsn S1 S2 t1 ->
     dbop S2 S3 t2 ->
     dbop S1 S3 (trace_app t1 t2)
-with dbFdef : id -> list_param -> State -> State -> trace -> Prop :=
-| dbFdef_intro : forall S M F B lc gl arg ExitValue rid t fid lp
-                            Oparg' arg' F' B' I' EC rt id la lb lc' state' tr,
-  params2OpGenericValues lp lc gl = Oparg' ->   
-  opGenericValues2GenericValues Oparg' = arg' ->   
-  lookupFdefViaIDFromSystemC S fid = Some F' ->
-  getEntryBlock F' = Some B' ->
+with dbFdef : id -> typ -> list_param -> system -> module -> list ExecutionContext -> GVMap -> GVMap -> GVMap -> GVMap -> block -> value -> trace -> Prop :=
+| dbFdef_intro : forall S M gl fid lp lc
+                            B' I' rt la lb B'' Result lc' gl' tr ECs,
+  lookupFdefViaIDFromSystemC S fid = Some (fdef_intro (fheader_intro rt fid la) lb) ->
+  getEntryBlock (fdef_intro (fheader_intro rt fid la) lb) = Some B' ->
   getEntryInsn B' = Some I' ->
-  F' = fdef_intro (fheader_intro rt id la) lb ->
-  initializeFrameValues la arg' = lc' ->
   dbop 
-    (mkState S M ExitValue ((mkEC F' B' I' lc' arg')::(mkEC F B (insn_call rid t fid lp) lc arg)::EC) gl)
-    state'
+    (mkState S M ((mkEC (fdef_intro (fheader_intro rt fid la) lb) 
+                             B' I' (initLocals la (params2GVs lp lc gl))
+                            (params2GVs lp lc gl))::ECs) gl)
+    (mkState S M ((mkEC (fdef_intro (fheader_intro rt fid la) lb) 
+                             B'' (insn_return rt Result) lc'
+                            (params2GVs lp lc gl))::ECs) gl')
     tr ->
-  dbFdef fid lp 
-    (mkState S M ExitValue ((mkEC F B (insn_call rid t fid lp) lc arg)::EC) gl) state' tr
+  dbFdef fid rt lp S M ECs lc gl lc' gl' B'' Result tr
 .
 
-CoInductive dbInstInf : State -> Trace -> Prop :=
-| dbCallInsntInf : forall S M F B lc gl arg rid t fid lp gl' gl''
-                       EC ExitValue ReturnValue tr I',
-  dbFdefInf fid lp
-    (mkState S M None ((mkEC F B (insn_call rid t fid lp) lc arg)::nil) gl) 
-    tr ->
-  updateGlobals gl' rid ReturnValue = gl'' -> 
-  getNextInsnFrom (insn_call rid t fid lp) B = Some I' ->
-  dbInstInf 
-    (mkState S M ExitValue ((mkEC F B (insn_call rid t fid lp) lc arg)::EC) gl) 
+CoInductive dbInsnInf : State -> Trace -> Prop :=
+| dbCallInsnInf : forall S M F B lc gl arg rid rt fid lp
+                       EC tr,
+  dbFdefInf fid rt lp S M ((mkEC F B (insn_call rid rt fid lp) lc arg)::EC) lc gl tr ->
+  dbInsnInf 
+    (mkState S M ((mkEC F B (insn_call rid rt fid lp) lc arg)::EC) gl) 
     tr
 with dbopInf : State -> Trace -> Prop :=
-| dbopInf_cons1 : forall S1 t1,
-    dbInstInf S1 t1 ->
-    dbopInf S1 t1
-| dbopInf_cons2 : forall S1 S2 t1 t2,
-    dbInst S1 S2 t1 ->
-    dbopInf S2 t2 ->
-    dbopInf S1 (Trace_app t1 t2)
-with dbFdefInf : id -> list_param -> State -> Trace -> Prop :=
-| dbFdefInf_intro : forall S M F B lc gl arg ExitValue rid t fid lp
-                            Oparg' arg' F' B' I' EC rt id la lb lc' tr,
-  params2OpGenericValues lp lc gl = Oparg' ->   
-  opGenericValues2GenericValues Oparg' = arg' ->   
-  lookupFdefViaIDFromSystemC S fid = Some F' ->
-  getEntryBlock F' = Some B' ->
+| dbopInf_insn : forall state1 t1,
+    dbInsnInf state1 t1 ->
+    dbopInf state1 t1
+| dbopInf_cons : forall state1 state2 t1 t2,
+    dbInsn state1 state2 t1 ->
+    dbopInf state2 t2 ->
+    dbopInf state1 (Trace_app t1 t2)
+with dbFdefInf : id -> typ -> list_param -> system -> module -> list ExecutionContext -> GVMap -> GVMap -> Trace -> Prop :=
+| dbFdefInf_intro : forall S M lc gl fid lp
+                           B' I' rt la lb tr ECs ,
+  lookupFdefViaIDFromSystemC S fid = Some (fdef_intro (fheader_intro rt fid la) lb) ->
+  getEntryBlock (fdef_intro (fheader_intro rt fid la) lb) = Some B' ->
   getEntryInsn B' = Some I' ->
-  F' = fdef_intro (fheader_intro rt id la) lb ->
-  initializeFrameValues la arg' = lc' ->
   dbopInf 
-    (mkState S M ExitValue ((mkEC F' B' I' lc' arg')::(mkEC F B (insn_call rid t fid lp) lc arg)::EC) gl)
+    (mkState S M ((mkEC (fdef_intro (fheader_intro rt fid la) lb) B' I' 
+                        (initLocals la (params2GVs lp lc gl)) 
+                        (params2GVs lp lc gl))::ECs) gl)
     tr ->
-  dbFdefInf fid lp 
-    (mkState S M ExitValue ((mkEC F B (insn_call rid t fid lp) lc arg)::EC) gl) 
-    tr
+  dbFdefInf fid rt lp S M ECs lc gl tr
 .
 
 Definition db_genInitState := ds_genInitState.
@@ -807,62 +742,30 @@ Inductive db_goeswrong : system -> id -> list GenericValue -> State -> Prop :=
 (***************************************************************)
 (* non-deterministic big-step *)
 
-Fixpoint returnStatesFromFdef S M (gls_ev_tr : list (GVMap*(option GenericValue)*trace)) : States :=
-match gls_ev_tr with
+Fixpoint returnStatesFromOp S M ECs lp lc gl rt fid la lb (lc_gl_block_re_trs : list (GVMap*GVMap*block*value*trace)) : States :=
+match lc_gl_block_re_trs with
 | nil => nil
-| (gl, ev, tr)::gls_ev_tr' => (mkState S M ev nil gl, tr)::(returnStatesFromFdef S M gls_ev_tr')
+| (lc', gl', B'', re, tr')::lc_gl_block_re_trs' => 
+    (mkState S M ((mkEC (fdef_intro (fheader_intro rt fid la) lb) 
+                             B'' (insn_return rt re) lc'
+                            (params2GVs lp lc gl))::ECs) gl', tr')::
+    (returnStatesFromOp S M ECs lp lc gl rt fid la lb lc_gl_block_re_trs')
 end.
 
-Fixpoint updateStatesFromReturns S M F B I' ExitValue lc arg EC rid gls_ev_tr : States :=
-match gls_ev_tr with 
+Fixpoint updateStatesFromReturns S M F B I' lc t arg EC rid (lc_gl_block_re_trs : list (GVMap*GVMap*block*value*trace)): States :=
+match lc_gl_block_re_trs with 
 | nil => nil
-| (gl, ev, tr)::gls_ev_tr' => 
-  (mkState S M ExitValue ((mkEC F B I' lc arg)::EC) (updateGlobals gl rid ev), tr)::
-  (updateStatesFromReturns S M F B I' ExitValue lc arg EC rid gls_ev_tr')
+| (lc', gl', B', re, tr)::lc_gl_block_re_trs' => 
+  let ogv := getOperandValue re lc' gl' in 
+  let (lc'', gl'') := (if (t =t= typ_void) 
+                      then (lc, gl') 
+                      else (updateMem lc gl' rid ogv)) in
+  (mkState S M ((mkEC F B I' lc'' arg)::EC) gl'', tr)::
+  (updateStatesFromReturns S M F B I' lc t arg EC rid lc_gl_block_re_trs')
 end.
 
-Inductive nbInst : State*trace -> States -> Prop :=
-| nbReturn_finished : forall S M F B RetTy Result lc gl arg ExitValue tr,
-  (* Finished main.  Put result into exit code... *)
-  ExitValue =  (if (Typ.isInteger RetTy)  (* Nonvoid return type? *)
-               then getOperandValue Result lc gl (* Capture the exit value of the program *)
-               else Some GV_undef) ->
-  nbInst 
-    (mkState S M None ((mkEC F B (insn_return RetTy Result) lc arg)::nil) gl, tr)
-    ((mkState S M ExitValue nil gl, tr)::nil)
-| nbReturn_call : forall S M F B RetTy Result lc gl arg id
-                            F' B' I' lc' arg' EC gv
-                            I'' lc'' gl'' tr,   
-  (* If we have a previous stack frame, and we have a previous call,
-          fill in the return value... *)
-  Instruction.isCallInst I' ->
-  getCallerReturnID I' = Some id ->
-  getOperandValue Result lc gl = Some gv -> 
-  (lc'', gl'') = (if (RetTy =t= typ_void) 
-                  then (lc', gl) 
-                  else (updateMem lc' gl id (Some gv))) ->
-  getNextInsnFrom I' B' = Some I'' ->
-  nbInst 
-    (mkState S M None ((mkEC F B (insn_return RetTy Result) lc arg)::(mkEC F' B' I' lc' arg')::EC) gl, tr)
-    ((mkState S M None ((mkEC F' B' I'' lc'' arg')::EC) gl'', tr)::nil)
-| nbReturnVoid_finished : forall S M F B lc gl arg ExitValue tr,
-  (* Finished main.  Put result into exit code... *)
-  ExitValue = Some GV_undef ->
-  nbInst 
-    (mkState S M None ((mkEC F B (insn_return_void) lc arg)::nil) gl, tr)
-    ((mkState S M ExitValue nil gl, tr)::nil)
-| nbReturnVoid_call : forall S M F B lc gl arg ExitValue id
-                            F' B' I' lc' arg' EC
-                            I'' tr,   
-  (* If we have a previous stack frame, and we have a previous call,
-          fill in the return value... *)
-  Instruction.isCallInst I' ->
-  getCallerReturnID I' = Some id ->
-  getNextInsnFrom I' B' = Some I'' ->
-  nbInst 
-    (mkState S M ExitValue ((mkEC F B insn_return_void lc arg)::(mkEC F' B' I' lc' arg')::EC) gl, tr)
-    ((mkState S M ExitValue ((mkEC F' B' I'' lc' arg')::EC) gl, tr)::nil)
-| nbBranch_def : forall S M F B lc gl arg ExitValue t Cond l1 l2 c
+Inductive nbInsn : State*trace -> States -> Prop :=
+| nbBranch_def : forall S M F B lc gl arg t Cond l1 l2 c
                               B' I' lc' Dest EC tr,   
   getOperandValue Cond lc gl = Some (GV_int c) ->
   Some Dest = (if c 
@@ -870,10 +773,10 @@ Inductive nbInst : State*trace -> States -> Prop :=
                else lookupBlockViaLabelFromSystem S l2) ->
   (B', lc') = (switchToNewBasicBlock Dest B lc) ->
   getEntryInsn B' = Some I' ->
-  nbInst 
-    (mkState S M ExitValue ((mkEC F B (insn_br t Cond l1 l2) lc arg)::EC) gl, tr)
-    ((mkState S M ExitValue ((mkEC F B' I' lc' arg)::EC) gl, tr)::nil)
-| nbBranch_undef : forall S M F B lc arg ExitValue t Cond l1 l2
+  nbInsn 
+    (mkState S M ((mkEC F B (insn_br t Cond l1 l2) lc arg)::EC) gl, tr)
+    ((mkState S M ((mkEC F B' I' lc' arg)::EC) gl, tr)::nil)
+| nbBranch_undef : forall S M F B lc arg t Cond l1 l2
                               B1' I1' lc1' B2' I2' lc2' Dest1 Dest2 EC tr gl,   
   getOperandValue Cond lc gl = Some GV_undef ->
   Some Dest1 = lookupBlockViaLabelFromSystem S l1 ->
@@ -882,62 +785,61 @@ Inductive nbInst : State*trace -> States -> Prop :=
   (B2', lc2') = (switchToNewBasicBlock Dest2 B lc) ->
   getEntryInsn B1' = Some I1' ->
   getEntryInsn B2' = Some I2' ->
-  nbInst 
-    (mkState S M ExitValue ((mkEC F B (insn_br t Cond l1 l2) lc arg)::EC) gl, tr)
-    ((mkState S M ExitValue ((mkEC F B1' I1' lc1' arg)::EC) gl, tr)::
-     (mkState S M ExitValue ((mkEC F B2' I2' lc2' arg)::EC) gl, tr)::nil)
-| nbBranch_uncond : forall S M F B lc gl arg ExitValue l
+  nbInsn 
+    (mkState S M ((mkEC F B (insn_br t Cond l1 l2) lc arg)::EC) gl, tr)
+    ((mkState S M ((mkEC F B1' I1' lc1' arg)::EC) gl, tr)::
+     (mkState S M ((mkEC F B2' I2' lc2' arg)::EC) gl, tr)::nil)
+| nbBranch_uncond : forall S M F B lc gl arg l
                               B' I' lc' Dest EC tr,   
   Some Dest = (lookupBlockViaLabelFromSystem S l) ->
   (B', lc') = (switchToNewBasicBlock Dest B lc) ->
   getEntryInsn B = Some I' ->
-  nbInst 
-    (mkState S M ExitValue ((mkEC F B (insn_br_uncond l) lc arg)::EC) gl, tr)
-    ((mkState S M ExitValue ((mkEC F B' I' lc' arg)::EC) gl, tr)::nil)
-| nbCallInsnt : forall S M F B lc gl arg ExitValue rid t fid lp
-                            EC tr gls_ev_tr I', 
-  nbFdef fid lp
-    (mkState S M None ((mkEC F B (insn_call rid t fid lp) lc arg)::nil) gl, tr) 
-    (returnStatesFromFdef S M gls_ev_tr) ->
-  getNextInsnFrom (insn_call rid t fid lp) B = Some I' ->
-  nbInst 
-    (mkState S M ExitValue ((mkEC F B (insn_call rid t fid lp) lc arg)::EC) gl, tr) 
-    (updateStatesFromReturns S M F B I' ExitValue lc arg EC rid gls_ev_tr)
-| nbAddInsnt : forall S M F B lc gl lc' gl' arg ExitValue id t v1 v2 EC i1 i2 I' tr,
+  nbInsn 
+    (mkState S M ((mkEC F B (insn_br_uncond l) lc arg)::EC) gl, tr)
+    ((mkState S M ((mkEC F B' I' lc' arg)::EC) gl, tr)::nil)
+| nbCallInsnt : forall S M F B lc gl arg rid rt fid lp
+                            EC tr lc_gl_block_re_trs I', 
+  nbFdef fid rt lp S M ((mkEC F B (insn_call rid rt fid lp) lc arg)::EC) lc gl tr lc_gl_block_re_trs ->
+  getNextInsnFrom (insn_call rid rt fid lp) B = Some I' ->
+  nbInsn 
+    (mkState S M ((mkEC F B (insn_call rid rt fid lp) lc arg)::EC) gl, tr) 
+    (updateStatesFromReturns S M F B I' lc rt arg EC rid lc_gl_block_re_trs)
+| nbAddInsnt : forall S M F B lc gl lc' gl' arg id t v1 v2 EC i1 i2 I' tr,
   getOperandValue v1 lc gl = Some (GV_int i1) ->
   getOperandValue v2 lc gl = Some (GV_int i2) ->
   getNextInsnFrom (insn_add id t v1 v2) B = Some I' ->
   updateMem lc gl id (Some (GV_int (i1+i2))) = (lc', gl') -> 
-  nbInst 
-    (mkState S M ExitValue ((mkEC F B (insn_add id t v1 v2) lc arg)::EC) gl, tr) 
-    ((mkState S M ExitValue ((mkEC F B I' lc' arg)::EC) gl', tr)::nil)
-with nbInstMerge : States -> States -> Prop :=
-| nbInstMerge_nil : nbInstMerge nil nil
-| nbInstMerge_cons : forall state tr states states1 states2,
-  nbInst (state, tr) states1 ->
-  nbInstMerge states states2 ->
-  nbInstMerge ((state, tr)::states) (states1++states2)
+  nbInsn 
+    (mkState S M ((mkEC F B (insn_add id t v1 v2) lc arg)::EC) gl, tr) 
+    ((mkState S M ((mkEC F B I' lc' arg)::EC) gl', tr)::nil)
+with nbInsnMerge : States -> States -> Prop :=
+| nbInsnMerge_nil : nbInsnMerge nil nil
+| nbInsnMerge_cons : forall state tr states states1 states2,
+  nbInsn (state, tr) states1 ->
+  nbInsnMerge states states2 ->
+  nbInsnMerge ((state, tr)::states) (states1++states2)
+| nbInsnMerge_final : forall state tr states states',
+  ds_isFinialState state ->
+  nbInsnMerge states states' ->
+  nbInsnMerge ((state, tr)::states) ((state, tr)::states')
 with nbop : States -> States -> Prop :=
 | nbop_nil : nbop nil nil
 | nbop_cons : forall states1 states2 states3,
-  nbInstMerge states1 states2 ->
+  nbInsnMerge states1 states2 ->
   nbop states2 states3 ->
   nbop states1 states3 
-with nbFdef : id -> list_param -> State*trace -> States -> Prop :=
-| nbFdef_intro : forall S M F B lc gl arg ExitValue rid t fid lp
-                            Oparg' arg' F' B' I' EC rt id la lb lc' states' tr,
-  params2OpGenericValues lp lc gl = Oparg' ->   
-  opGenericValues2GenericValues Oparg' = arg' ->   
-  lookupFdefViaIDFromSystemC S fid = Some F' ->
-  getEntryBlock F' = Some B' ->
+with nbFdef : id -> typ -> list_param -> system -> module -> list ExecutionContext -> GVMap -> GVMap -> trace -> list (GVMap*GVMap*block*value*trace) -> Prop :=
+| nbFdef_intro : forall S M lc gl fid lp
+                            B' I' rt la lb tr lc_gl_block_re_trs ECs,
+  lookupFdefViaIDFromSystemC S fid = Some (fdef_intro (fheader_intro rt fid la) lb) ->
+  getEntryBlock (fdef_intro (fheader_intro rt fid la) lb) = Some B' ->
   getEntryInsn B' = Some I' ->
-  F' = fdef_intro (fheader_intro rt id la) lb ->
-  initializeFrameValues la arg' = lc' ->
   nbop 
-    ((mkState S M ExitValue ((mkEC F' B' I' lc' arg')::(mkEC F B (insn_call rid t fid lp) lc arg)::EC) gl, tr)::nil)
-    states' ->
-  nbFdef fid lp 
-    (mkState S M ExitValue ((mkEC F B (insn_call rid t fid lp) lc arg)::EC) gl, tr) states'
+    ((mkState S M ((mkEC (fdef_intro (fheader_intro rt fid la) lb) 
+                         B' I' (initLocals la (params2GVs lp lc gl)) 
+                         (params2GVs lp lc gl))::ECs) gl, tr)::nil)
+    (returnStatesFromOp S M ECs lp lc gl rt fid la lb lc_gl_block_re_trs) ->
+  nbFdef fid rt lp S M ECs lc gl tr lc_gl_block_re_trs
 .
 
 Definition StatesInf := list (State*Trace).
@@ -950,45 +852,41 @@ Inductive wfStatesInf : StatesInf -> Prop :=
   wfStatesInf ((state, t)::states)
 .
 
-CoInductive nbInstInf : State*trace -> list Trace -> Prop :=
-| nbCallInsntInf : forall S M F B lc gl arg ExitValue rid t fid lp
+CoInductive nbInsnInf : State*trace -> list Trace -> Prop :=
+| nbCallInsnInf : forall S M F B lc gl arg rid rt fid lp
                             EC tr trs, 
-  nbFdefInf fid lp
-    (mkState S M None ((mkEC F B (insn_call rid t fid lp) lc arg)::nil) gl, tr) 
-    trs ->
-  nbInstInf 
-    (mkState S M ExitValue ((mkEC F B (insn_call rid t fid lp) lc arg)::EC) gl, tr)
+  nbFdefInf fid rt lp S M 
+    ((mkEC F B (insn_call rid rt fid lp) lc arg)::nil)      
+    lc gl tr trs ->
+  nbInsnInf 
+    (mkState S M ((mkEC F B (insn_call rid rt fid lp) lc arg)::EC) gl, tr)
     trs
-with nbInstInfMerge : States -> list Trace -> Prop :=
-| nbInstInfMerge_nil : nbInstInfMerge nil nil
-| nbInstInfMerge_cons : forall state states tr1 tr2,
-  nbInstInf state tr1 ->
-  nbInstInfMerge states tr2 ->
-  nbInstInfMerge (state::states) (tr1++tr2)
+with nbInsnInfMerge : States -> list Trace -> Prop :=
+| nbInsnInfMerge_nil : nbInsnInfMerge nil nil
+| nbInsnInfMerge_cons : forall state states tr1 tr2,
+  nbInsnInf state tr1 ->
+  nbInsnInfMerge states tr2 ->
+  nbInsnInfMerge (state::states) (tr1++tr2)
 with nbopInf : States -> list Trace -> Prop :=
 | nbopInf_cons1 : forall states trs,
-  nbInstInfMerge states trs ->
+  nbInsnInfMerge states trs ->
   nbopInf states trs
 | nbopInf_cons2 : forall states1 states2 states3,
-  nbInstMerge states1 states2 ->
+  nbInsnMerge states1 states2 ->
   nbopInf states2 states3 ->
   nbopInf states1 states3 
-with nbFdefInf : id -> list_param -> State*trace -> list Trace -> Prop :=
-| nbFdefInf_intro : forall S M F B lc gl arg ExitValue rid t fid lp
-                            Oparg' arg' F' B' I' EC rt id la lb lc' tr tr',
-  params2OpGenericValues lp lc gl = Oparg' ->   
-  opGenericValues2GenericValues Oparg' = arg' ->   
-  lookupFdefViaIDFromSystemC S fid = Some F' ->
-  getEntryBlock F' = Some B' ->
+with nbFdefInf : id -> typ -> list_param -> system -> module -> list ExecutionContext -> GVMap -> GVMap -> trace -> list Trace -> Prop :=
+| nbFdefInf_intro : forall S M lc gl fid lp
+                            B' I' ECs rt la lb tr tr',
+  lookupFdefViaIDFromSystemC S fid = Some (fdef_intro (fheader_intro rt fid la) lb) ->
+  getEntryBlock (fdef_intro (fheader_intro rt fid la) lb) = Some B' ->
   getEntryInsn B' = Some I' ->
-  F' = fdef_intro (fheader_intro rt id la) lb ->
-  initializeFrameValues la arg' = lc' ->
   nbopInf 
-    ((mkState S M ExitValue ((mkEC F' B' I' lc' arg')::(mkEC F B (insn_call rid t fid lp) lc arg)::EC) gl, tr)::nil) 
+    ((mkState S M ((mkEC (fdef_intro (fheader_intro rt fid la) lb) 
+                          B' I' (initLocals la (params2GVs lp lc gl)) 
+                          (params2GVs lp lc gl))::ECs) gl, tr)::nil) 
     tr' ->
-  nbFdefInf fid lp 
-    (mkState S M ExitValue ((mkEC F B (insn_call rid t fid lp) lc arg)::EC) gl, tr)
-    tr'
+  nbFdefInf fid rt lp S M ECs lc gl tr tr'
 .
 
 Definition nb_genInitState := ns_genInitState.
@@ -1016,6 +914,31 @@ Inductive nb_goeswrong : system -> id -> list GenericValue -> States -> Prop :=
   ~ nb_isFinialState FS ->
   nb_goeswrong s main VarArgs FS
 .
+
+Scheme dbInsn_ind2 := Induction for dbInsn Sort Prop
+  with dbop_ind2 := Induction for dbop Sort Prop
+  with dbFdef_ind2 := Induction for dbFdef Sort Prop.
+
+Combined Scheme db_mutind from dbInsn_ind2, dbop_ind2, dbFdef_ind2.
+
+Tactic Notation "db_mutind_cases" tactic(first) tactic(c) :=
+  first;
+  [ c "dbBranch" | c "dbBranch_uncond" | c "dbCallInsn" |
+    c "dbAddInsn" | c "dbop_nil" | c "dbop_cons" |
+    c "dbFdef_intro" ].
+
+Tactic Notation "dsInsn_cases" tactic(first) tactic(c) :=
+  first;
+  [ c "dsReturn" | c "dsBranch" | c "dsBranch_uncond" | c "dsCallInsn" |
+    c "dsAddInsn" ].
+
+Tactic Notation "dsop_star_cases" tactic(first) tactic(c) :=
+  first;
+  [ c "dsop_star_nil" | c "dsop_star_cons" ].
+
+Hint Constructors dbInsn dbop dbFdef.
+Hint Constructors dsInsn dsop_star dsop_diverges dsop_plus.
+
 
 (*****************************)
 (*
