src/ssa/llvm_op/ssa_verifier.v
@@ -534,9 +534,11 @@ Inductive wf_insn : intrinsic_funs -> system -> module_info -> fdef_info -> bloc
  | wf_insn_return : forall (intrinsic_funs5:intrinsic_funs) (system5:system) (module_info5:module_info) (fdef5:fdef) (dt5:dt) (block5:block) (typ5:typ) (value5:value),
      visitReturnInst intrinsic_funs5 system5 module_info5   ( fdef5 ,  dt5 )   block5 (insn_return typ5 value5) ->
      wf_insn intrinsic_funs5 system5 module_info5   ( fdef5 ,  dt5 )   block5 (insn_return typ5 value5)
+(*
  | wf_insn_return_void : forall (intrinsic_funs5:intrinsic_funs) (system5:system) (module_info5:module_info) (fdef5:fdef) (dt5:dt) (block5:block),
      visitReturnInst intrinsic_funs5 system5 module_info5   ( fdef5 ,  dt5 )   block5 insn_return_void ->
      wf_insn intrinsic_funs5 system5 module_info5   ( fdef5 ,  dt5 )   block5 insn_return_void
+*)
  | wf_insn_br : forall (intrinsic_funs5:intrinsic_funs) (system5:system) (module_info5:module_info) (block5:block) (typ5:typ) (value5:value) (l1 l2:l) (fdef5:fdef) (dt5:dt) ,
      typ5 =t= (typ_int 1) ->
      visitTerminatorInst intrinsic_funs5 system5 module_info5   ( fdef5 ,  dt5 )   block5 (insn_br typ5 value5 l1 l2) ->
