src/ssa/opsem_conv.v
@@ -1,0 +1,402 @@
+Add LoadPath "./ott".
+Add LoadPath "./monads".
+Require Import ssa_dynamic.
+Require Import ssa.
+Require Import List.
+Require Import tactics.
+
+(***********************************************************)
+(** trace and Trace                                        *)
+
+Lemma trace_app_nil__eq__trace : forall tr,
+  trace_app tr trace_nil = tr.
+Proof.
+  induction tr; simpl; auto.
+    rewrite IHtr. auto.
+Qed.
+
+Lemma nil_app_trace__eq__trace : forall tr,
+  trace_app trace_nil tr = tr.
+Proof. auto. Qed.
+
+Lemma trace_app_commute : forall tr1 tr2 tr3,
+  trace_app tr1 (trace_app tr2 tr3) = trace_app (trace_app tr1 tr2) tr3.
+Proof.
+  induction tr1; intros; simpl; auto.
+    rewrite IHtr1. auto.
+Qed.
+
+Lemma nil_app_Trace__eq__Trace : forall tr,
+  Trace_app trace_nil tr = tr.
+Proof. auto. Qed.
+
+Lemma Trace_app_commute : forall tr1 tr2 tr3,
+  Trace_app tr1 (Trace_app tr2 tr3) = Trace_app (trace_app tr1 tr2) tr3.
+Proof.
+  induction tr1; intros; simpl; auto.
+    rewrite IHtr1. auto.
+Qed.
+
+(***********************************************************)
+(** det small-step                                         *)
+
+Lemma dsInsn__implies__dsop_star : forall state state' tr,
+  dsInsn state state' tr ->
+  dsop_star state state' tr.
+Proof.
+  intros state state' tr HdsInsn.
+  rewrite <- trace_app_nil__eq__trace.
+  eapply dsop_star_cons; eauto.
+Qed.
+
+Lemma dsInsn__implies__dsop_plus : forall state state' tr,
+  dsInsn state state' tr ->
+  dsop_plus state state' tr.
+Proof.
+  intros state state' tr HdsInsn.
+  rewrite <- trace_app_nil__eq__trace.
+  eapply dsop_plus_cons; eauto.
+Qed.
+
+Lemma dsop_plus__implies__dsop_star : forall state state' tr,
+  dsop_plus state state' tr ->
+  dsop_star state state' tr.
+Proof.
+  intros state state' tr dsop_plus.
+  inversion dsop_plus; subst; eauto.
+Qed.
+
+Hint Resolve dsInsn__implies__dsop_star dsInsn__implies__dsop_plus dsop_plus__implies__dsop_star. 
+
+Lemma dsop_star_trans : forall state1 state2 state3 tr12 tr23,
+  dsop_star state1 state2 tr12 ->
+  dsop_star state2 state3 tr23 ->
+  dsop_star state1 state3 (trace_app tr12 tr23).
+Proof.
+  intros state1 state2 state3 tr12 tr23 Hdsop12 Hdsop23.
+  generalize dependent state3.
+  generalize dependent tr23.
+  induction Hdsop12; intros; auto.
+    rewrite <- trace_app_commute.
+    apply dsop_star_cons with (state2:=state2); auto.
+Qed.
+
+Lemma dsop_diverging_trans : forall state tr1 state' tr2,
+  dsop_star state state' tr1 ->
+  dsop_diverges state' tr2 ->
+  dsop_diverges state (Trace_app tr1 tr2).
+Proof. 
+  intros state tr1 state' tr2 state_dsop_state' state'_dsop_diverges.
+  generalize dependent tr2.
+  (dsop_star_cases (induction state_dsop_state') Case); intros; auto.
+  Case "dsop_star_cons".
+    rewrite <- Trace_app_commute.
+    apply dsop_diverges_intro with (state2:=state2); auto.
+Qed.
+
+(***********************************************************)
+(** det big-step convergence -> det small-step convergence *)
+
+(** First, by mutual induction, we prove that dbInsn, dbop and  
+    dbFdef imply small-step semantics. *)
+
+Definition dbInsn__implies__dsop_plus_prop state state' tr (db:dbInsn state state' tr) := 
+  dsop_plus state state' tr.
+Definition dbop__implies__dsop_star_prop state state' tr (db:dbop state state' tr) := 
+  dsop_star state state' tr.
+Definition dbFdef__implies__dsop_star_prop fid rt lp S M ECs lc gl lc' gl' B'' Result tr 
+           (db:dbFdef fid rt lp S M ECs lc gl lc' gl' B'' Result tr) := 
+  forall B' I' la lb,
+  lookupFdefViaIDFromSystemC S fid = Some (fdef_intro (fheader_intro rt fid la) lb) ->
+  getEntryBlock (fdef_intro (fheader_intro rt fid la) lb) = Some B' ->
+  getEntryInsn B' = Some I' ->
+  dsop_star
+    (mkState S M ((mkEC (fdef_intro (fheader_intro rt fid la) lb) 
+                             B' I' (initLocals la (params2GVs lp lc gl))
+                            (params2GVs lp lc gl))::ECs) gl)
+    (mkState S M ((mkEC (fdef_intro (fheader_intro rt fid la) lb) 
+                             B'' (insn_return rt Result) lc'
+                            (params2GVs lp lc gl))::ECs) gl')
+    tr
+  .
+
+Lemma db__implies__ds:
+  (forall state state' t  db, @dbInsn__implies__dsop_plus_prop state state' t db) /\
+  (forall state state' t  db, @dbop__implies__dsop_star_prop state state' t db) /\
+  (forall fid rt lp S M ECs lc gl lc' gl' B'' ret tr db, 
+     @dbFdef__implies__dsop_star_prop fid rt lp S M ECs lc gl lc' gl' B'' ret tr db).
+Proof.
+(db_mutind_cases
+  apply db_mutind with
+    (P  := dbInsn__implies__dsop_plus_prop)
+    (P0 := dbop__implies__dsop_star_prop)
+    (P1 := dbFdef__implies__dsop_star_prop)
+    Case);
+  unfold dbInsn__implies__dsop_plus_prop, 
+         dbop__implies__dsop_star_prop, 
+         dbFdef__implies__dsop_star_prop; 
+  intros; subst; simpl; intuition; eauto.
+  Case "dbCallInsn".
+    inversion d. subst.
+    assert (Hlookup:=H0).
+    apply H with (B'0:=B'0)(I':=I'0) in H0; auto.
+    rewrite <- nil_app_trace__eq__trace.
+    apply dsop_plus_cons with 
+      (state2:=mkState S M ((mkEC (fdef_intro (fheader_intro rt fid la) lb)
+                               B'0 I'0 (initLocals la (params2GVs lp lc gl)) 
+                               (params2GVs lp lc gl))::
+                        (mkEC F B (insn_call rid rt fid lp) lc arg)::EC) 
+                        gl); auto.
+    rewrite <- trace_app_nil__eq__trace.
+    apply dsop_star_trans with 
+      (state2:=mkState S M ((mkEC (fdef_intro (fheader_intro rt fid la) lb) 
+                               B' (insn_return rt Result) lc'
+                               (params2GVs lp lc gl))::
+                        (mkEC F B (insn_call rid rt fid lp) lc arg)::EC) 
+                        gl'); auto.
+      apply dsInsn__implies__dsop_star.
+      eapply dsReturn; simpl; eauto.
+  
+  Case "dbop_cons".
+    apply dsop_star_trans with (state2:=S2); auto.
+        
+  Case "dbFdef_intro".
+    rewrite H0 in e. inversion e; subst.
+    rewrite H1 in e0. inversion e0; subst.
+    rewrite H2 in e1. inversion e1; subst.
+    exact H.
+Qed.  
+    
+Lemma dbInsn__implies__dsop_plus : forall state state' tr,
+  dbInsn state state' tr ->
+  dsop_plus state state' tr.
+Proof.
+  destruct db__implies__ds as [J _]. eauto.
+Qed.
+
+Lemma dbInsn__implies__dsop_star : forall state state' tr,
+  dbInsn state state' tr ->
+  dsop_star state state' tr.
+Proof. 
+  intros state state' tr state_dbInsn_state'.
+  apply dbInsn__implies__dsop_plus in state_dbInsn_state'; auto.
+Qed.
+
+Lemma dbop__implies__dsop_star : forall state state' tr,
+  dbop state state' tr ->
+  dsop_star state state' tr.
+Proof.
+  destruct db__implies__ds as [_ [J _]]. eauto.
+Qed.
+
+Lemma dbFdef__implies__dsop_star : forall fid rt lp S M ECs lc gl lc' gl' B'' Result tr B' I' la lb,
+  dbFdef fid rt lp S M ECs lc gl lc' gl' B'' Result tr ->
+  lookupFdefViaIDFromSystemC S fid = Some (fdef_intro (fheader_intro rt fid la) lb) ->
+  getEntryBlock (fdef_intro (fheader_intro rt fid la) lb) = Some B' ->
+  getEntryInsn B' = Some I' ->
+  dsop_star 
+    (mkState S M ((mkEC (fdef_intro (fheader_intro rt fid la) lb) 
+                             B' I' (initLocals la (params2GVs lp lc gl))
+                            (params2GVs lp lc gl))::ECs) gl)
+    (mkState S M ((mkEC (fdef_intro (fheader_intro rt fid la) lb) 
+                             B'' (insn_return rt Result) lc'
+                            (params2GVs lp lc gl))::ECs) gl')
+    tr.
+Proof.
+  intros fid rt lp S M EC lc gl lc' gl' B'' Result tr B' I' la lb H.
+  revert fid rt lp S M EC lc gl lc' gl' B'' Result tr H B' I' la lb.
+  destruct db__implies__ds as [_ [_ J]]. eauto.
+Qed.
+
+(** Then we prove that the whole program holds the same property. *)
+
+Lemma db_converges__implies__ds_converges : forall sys main VarArgs FS,
+  db_converges sys main VarArgs FS ->
+  ds_converges sys main VarArgs FS.
+Proof.
+  intros sys main VarArgs FS Hdb_converges.
+  inversion Hdb_converges; subst.
+  apply ds_converges_intro with (IS:=IS)(tr:=tr); auto.
+  apply dbop__implies__dsop_star; auto.
+Qed.
+
+Lemma db_goeswrong__implies__ds_goeswrong : forall sys main VarArgs FS,
+  db_goeswrong sys main VarArgs FS ->
+  ds_goeswrong sys main VarArgs FS.
+Proof.
+  intros sys main VarArgs FS Hdb_converges.
+  inversion Hdb_converges; subst.
+  apply ds_goeswrong_intro with (IS:=IS)(tr:=tr); auto.
+  apply dbop__implies__dsop_star; auto.
+Qed.
+
+(***********************************************************)
+(** det big-step convergence -> det small-step convergence *)
+
+(** First,we prove that dbInsn, dbop and dbFdef imply small-step semantics,
+    by nested coinduction. *)
+
+Lemma dbFdefInf__implies__dsop_diverges : forall fid rt lp S M ECs lc gl tr B' I' la lb,
+  dbFdefInf fid rt lp S M ECs lc gl tr ->
+  lookupFdefViaIDFromSystemC S fid = Some (fdef_intro (fheader_intro rt fid la) lb) ->
+  getEntryBlock (fdef_intro (fheader_intro rt fid la) lb) = Some B' ->
+  getEntryInsn B' = Some I' ->
+  dsop_diverges 
+    (mkState S M ((mkEC (fdef_intro (fheader_intro rt fid la) lb) B' I' 
+                        (initLocals la (params2GVs lp lc gl)) 
+                        (params2GVs lp lc gl))::ECs) gl)
+    tr.
+Proof.
+  cofix CIH_dbFdefInf.
+
+  assert (forall state tr, 
+          dbInsnInf state tr -> 
+          dsop_diverges state tr) as dbInsnInf__implies__dsop_diverges.
+    cofix CIH_dbInsnInf.
+    intros state tr HdbInsnInf.
+    
+    inversion HdbInsnInf; subst.
+    rewrite <- nil_app_Trace__eq__Trace.
+    assert (HdbFdefInf:=H).
+    inversion H; subst.
+    apply dsop_diverges_intro with 
+      (state2:=mkState S M ((mkEC (fdef_intro (fheader_intro rt fid la) lb)
+                               B' I' (initLocals la (params2GVs lp lc gl)) 
+                               (params2GVs lp lc gl))::
+                        (mkEC F B (insn_call rid rt fid lp) lc arg)::EC) 
+                        gl); 
+      try solve [clear CIH_dbFdefInf CIH_dbInsnInf; auto].
+      apply CIH_dbFdefInf with (B':=B')(I':=I')(la:=la)(lb:=lb) in HdbFdefInf; auto.
+
+  assert (forall state tr, 
+          dbopInf state tr -> 
+          dsop_diverges state tr) as dbopInf__implies__dsop_diverges.
+    cofix CIH_dbopInf.
+    intros state tr HdbopInf.
+    inversion HdbopInf; subst.
+    Case "dbopInf_insn".
+      apply dbInsnInf__implies__dsop_diverges in H; auto.
+    Case "dbopInf_cons".
+      apply dbInsn__implies__dsop_plus in H.
+      inversion H; subst.
+      SCase "dsop_plus_cons".
+        apply CIH_dbopInf in H0. clear CIH_dbopInf.
+        apply dsop_diverges_intro with (state2:=state2); auto.
+
+  intros fid rt lp S M ECs lc gl tr B' I' la lb 
+    HdbFdefInf Hlookup HgetEntryBlock HgetEntryInsn.
+  inversion HdbFdefInf; subst.
+  rewrite Hlookup in H. inversion H; subst.
+  rewrite HgetEntryBlock in H0. inversion H0; subst.
+  rewrite HgetEntryInsn in H1. inversion H1; subst.
+  apply dbopInf__implies__dsop_diverges in H2.
+  exact H2.
+Qed.
+
+Lemma dbInsnInf__implies__dsop_diverges : forall state tr, 
+  dbInsnInf state tr -> dsop_diverges state tr.
+Proof.
+  cofix CIH_dbInsnInf.
+  intros state tr HdbInsnInf.
+    
+  inversion HdbInsnInf; subst.
+  rewrite <- nil_app_Trace__eq__Trace.
+  assert (HdbFdefInf:=H).
+  inversion H; subst.
+  apply dsop_diverges_intro with 
+    (state2:=mkState S M ((mkEC (fdef_intro (fheader_intro rt fid la) lb)
+                             B' I' (initLocals la (params2GVs lp lc gl)) 
+                             (params2GVs lp lc gl))::
+                      (mkEC F B (insn_call rid rt fid lp) lc arg)::EC) 
+                      gl); 
+    try solve [clear CIH_dbInsnInf; auto].
+    apply dbFdefInf__implies__dsop_diverges with (B':=B')(I':=I')(la:=la)(lb:=lb) in HdbFdefInf; auto.
+Qed.
+
+Lemma dbopInf__implies__dsop_diverges : forall state tr, 
+  dbopInf state tr -> dsop_diverges state tr.
+Proof.
+  cofix CIH_dbopInf.
+  intros state tr HdbopInf.
+  inversion HdbopInf; subst.
+  Case "dbopInf_insn".
+    apply dbInsnInf__implies__dsop_diverges in H; auto.
+  Case "dbopInf_cons".
+    apply dbInsn__implies__dsop_plus in H.
+    inversion H; subst.
+    SCase "dsop_plus_cons".
+      apply CIH_dbopInf in H0. clear CIH_dbopInf.
+      apply dsop_diverges_intro with (state2:=state2); auto.
+Qed.
+
+(** Then we prove that the whole program holds the same property. *)
+
+Lemma db_diverges__implies__ds_diverges : forall sys main VarArgs,
+  db_diverges sys main VarArgs ->
+  ds_diverges sys main VarArgs.
+Proof.
+  intros sys main VarArgs Hdb_diverges.
+  inversion Hdb_diverges; subst.
+  apply ds_diverges_intro with (IS:=IS)(tr:=tr); auto.
+  apply dbopInf__implies__dsop_diverges; auto.
+Qed.
+
+(***********************************************************)
+(** misc *)
+
+(** We cannot prove tr1 and tr2 are equal, because the Leibniz
+    equivalence is too strong to reason about infinite objects.
+    We should prove tr1 and tr2 are bisimilar, but we also need
+    to change semantics with bisimilarity closure. We dont have
+    interesting traces now, so we leave this as future work.
+*)
+Lemma Trace_eq_head__eq_tail : forall tr tr1 tr2,
+  Trace_app tr tr1 = Trace_app tr tr2 ->
+  tr1 = tr2.
+Proof.
+Admitted.
+
+(** Potentially useful when proving small-step -> bigstep.
+*)
+Lemma dbopInf__dsInsn_dbopInf : forall state tr,
+  dbopInf state tr ->
+  exists state', exists tr1, exists tr2,
+    dsInsn state state' tr1 /\ dbopInf state' tr2 /\ Trace_app tr1 tr2 = tr.
+Proof.
+  intros state tr state_dbopInf.
+  inversion state_dbopInf; subst.
+Admitted.
+
+Lemma dsInsn_derministic : forall state state1 state2 tr1 tr2,
+  dsInsn state state1 tr1 ->
+  dsInsn state state2 tr2 ->
+  state1 = state2 /\ tr1 = tr2.
+Proof.
+  intros state state1 state2 tr1 tr2 HdsInsn1.
+  generalize dependent state2.
+  generalize dependent tr2.
+  (dsInsn_cases (induction HdsInsn1) Case); intros tr2 state2 HdsInsn2.
+  Case "dsReturn".
+    (dsInsn_cases (destruct HdsInsn2) SCase); auto.
+    SCase "dsReturn".
+Admitted.
+
+Lemma dsop_diverging__im_dsop_diverging : forall state tr1 state' tr2,
+  dsop_diverges state (Trace_app tr1 tr2) ->
+  dsop_star state state' tr1 ->
+  dsop_diverges state' tr2.
+Proof.
+  intros state tr1 state' tr2 state_dsop_diverges state_dsop_state'.
+  induction state_dsop_state'; auto.
+    apply IHstate_dsop_state'; auto.
+    rewrite <- Trace_app_commute in state_dsop_diverges.
+    inversion state_dsop_diverges; subst.
+    inversion H1; subst.
+    apply dsInsn_derministic with (state2:=state2)(tr2:=tr1) in H2; auto.
+    destruct H2; subst.
+    rewrite <- Trace_app_commute in H0.
+    apply Trace_eq_head__eq_tail in H0; subst.
+    rewrite <- H0.
+    apply dsop_diverging_trans with (state':=state4)(tr1:=tr6); auto.
+Qed.
+
